examples/dev/sw/examples/examples.sml
@@ -5,7 +5,8 @@
 use "compiler";
 
 (*---------------------------------------------------------------------------*)
-(* Addition 	                                                             *)
+(* Example 1: A simple program						     *)
+(* It implements the addition of two word32s                                 *)
 (*---------------------------------------------------------------------------*)
 
 val test1_def = Define
@@ -15,6 +16,41 @@ val test1_def = Define
                 (k1,k2)
             )
     `;
+(*
+  Name              : test1
+  Arguments         : r0 r1 
+  Modified Registers: r0 r2 
+  Returns           : r2 r0 
+  Body: 
+    0:          mov     ip, sp
+    1:          stmfd   sp!, {fp,ip,lr,pc}
+    2:          sub     fp, ip, #1i
+    3:          add     r2, r0, r1
+    4:          sub     r0, r0, r1
+    5:          sub     sp, fp, #3i
+    6:          ldmfd   sp, {fp,sp,pc}
+
+  Initial goal:
+         !pc0 cpsr0 regs0 pc1 cpsr1 regs1 mems1.
+           ((regs0 ' 14 = 7w) /\ (regs0 ' 13 = 100w) /\ (pc0 = 0) /\
+            terminated (instB,7) (pc0,cpsr0,regs0,mems0)) /\
+           ((pc1,cpsr1,regs1,mems1) =
+            terRun (instB,7) (pc0,cpsr0,regs0,mems0)) ==>
+           (pc1 = 7) /\
+           ((regs1 ' 2,regs1 ' 0) = test1 (regs0 ' 0,regs0 ' 1))
+
+  val arm1 = link2 test1_def;
+  
+  simT (mk_ARM arm1);
+
+  SEQ_TAC [test1_def];
+  
+*)
+
+(*---------------------------------------------------------------------------*)
+(* Example 2: A functions calls another function                             *)
+(* The proving is performed by "unrolling" the callee                        *)
+(*---------------------------------------------------------------------------*)
 
 val test2_def = Define
   `test2 (t1:word32,t2:word32) =
@@ -24,54 +60,92 @@ val test2_def = Define
             )
     `;
 
-
-val test3_def = Define
-  `test3 (t1:word32,t2:word32,t3:word32,t4:word32,t5:word32,t6:word32) =
-            (let k1 = UNCURRY $+ (t1,t5) in
-	     let (k2,k3) = test1 (k1, t6) in
-                (k2,k3)
-            )
-    `;
-
-
-
-(*
-    val arm1 = link2 test1_def;
-
-Arguments:
-    r0 r1
-Body:
+(******************************************************************
+  Name              : test2
+  Arguments         : r0 r1 
+  Modified Registers: r0 r1 
+  Returns           : r0 
+  Body: 
     0:          mov     ip, sp
     1:          stmfd   sp!, {fp,ip,lr,pc}
-    2:          sub     fp, ip, #1
-    3:          add     r2, r0, r1
-    4:          sub     r0, r0, r1
-    5:          sub     sp, fp, #2
-    6:          ldmfd   sp, {fp,sp,pc}
-Return:
-    r2 r0 
+    2:          sub     fp, ip, #1i
+    3:          sub     sp, sp, #2i
+    4:          stmfd   sp!, {r0,r1}
+    5:          bl      + (7)
+    6:          add     sp, sp, #2i
+    7:          ldmfd   sp, {r1,r0}
+    8:          add     sp, sp, #2i
+    9:          mul     r0, r1, r0
+   10:          sub     sp, fp, #3i
+   11:          ldmfd   sp, {fp,sp,pc}
+  *****************************************************************
+  Name              : test1
+  Arguments         : r0 r1 
+  Modified Registers: r0 r2 
+  Returns           : r2 r0 
+  Body: 
+   12:          mov     ip, sp
+   13:          stmfd   sp!, {r0,r2,fp,ip,lr,pc}
+   14:          sub     fp, ip, #1i
+   15:          ldmfd   ip, {r0,r1}
+   16:          add     r2, r0, r1
+   17:          sub     r0, r0, r1
+   18:          add     sp, fp, #5i
+   19:          stmfd   sp!, {r2,r0}
+   20:          sub     sp, fp, #5i
+   21:          ldmfd   sp, {r0,r2,fp,sp,pc}
 
-Initial goal:
-         !pc0 cpsr0 regs0 mems0.
-           (regs0 14 = 7w) /\ (regs0 13 = 100w) /\ (pc0 = 0) /\
-           terminated (instB,7) (pc0,cpsr0,regs0,mems0) ==>
-           (let (pc1,cpsr1,regs1,mems1) =
-                  terRun (instB,7) (pc0,cpsr0,regs0,mems0)
-            in
-              ((pc1 = 7) /\ T) /\
-              ((read (regs1,mems1) (REG 2),read (regs1,mems1) (REG 0)) =
-               test1
-                 (read (regs0,mems0) (REG 0),read (regs0,mems0) (REG 1))))
+  or,
 
+  print_structure := false
+ 
+  *****************************************************************
+  Name              : test2
+  Arguments         : r0 r1 
+  Modified Registers: r0 r1 
+  Returns           : r0 
+  Body: 
+    0:          mov     ip, sp
+    1:          stmfd   sp!, {fp,ip,lr,pc}
+    2:          sub     fp, ip, #1i
+    3:          sub     sp, sp, #2i
+    4:          stmfd   sp!, {r0,r1}
+    5:          bl      + (7)
+    6:          add     sp, sp, #2i
+    7:          ldmfd   sp, {r1,r0}
+    8:          add     sp, sp, #2i
+    9:          mul     r0, r1, r0
+   10:          sub     sp, fp, #3i
+   11:          ldmfd   sp, {fp,sp,pc}
+   12:          mov     ip, sp
+   13:          stmfd   sp!, {r0,r2,fp,ip,lr,pc}
+   14:          sub     fp, ip, #1i
+   15:          ldmfd   ip, {r0,r1}
+   16:          add     r2, r0, r1
+   17:          sub     r0, r0, r1
+   18:          add     sp, fp, #5i
+   19:          stmfd   sp!, {r2,r0}
+   20:          sub     sp, fp, #5i
+   21:          ldmfd   sp, {r0,r2,fp,sp,pc}
 
-    simT (mk_ARM arm1);
+  val arm2 = link2 test2_def;
+  simT (mk_ARM arm2);
 
-    ARM_TAC [test1_def];
-
+  SEQ_TAC [test1_def, test2_def]  
+  
 *)
 
+
 (*---------------------------------------------------------------------------*)
-(* Factorial Function                                                        *)
+(* Example 3: Conditional Jumps                                              *)
+(*                                  					     *)
+(*---------------------------------------------------------------------------*)
+
+
+
+(*---------------------------------------------------------------------------*)
+(* Example 4: Tail Recursive Functions					     *)
+(* This example works on the Factorial Function                              *)
 (*---------------------------------------------------------------------------*)
 
 val (f6_def, f6_ind) = Defn.tprove
@@ -80,44 +154,36 @@ val (f6_def, f6_ind) = Defn.tprove
    `f6 (x,a) = if x=0w then a else f6(x-1w,x*a)`,
   WF_REL_TAC `measure (w2n o FST)` THEN METIS_TAC [WORD_PRED_THM] );
 
-(*
-Arguments:
-    r0 r1
-Body:
+(******************************************************************
+  Name              : f6
+  Arguments         : r0 r1 
+  Modified Registers: r0 r2 r3 
+  Returns           : r0 
+  Body: 
     0:          mov     ip, sp
     1:          stmfd   sp!, {fp,ip,lr,pc}
-    2:          sub     fp, ip, #1
-    3:          mov     r2, #0w
-    4:          cmp     r0, r2
-    5:          beq     + (8)
-    6:          mov     r2, #1w
-    7:          sub     r3, r0, r2
-    8:          mul     r2, r0, r1
-    9:          stmfd   sp!, {r3,r2}
-   10:          ldmfd   sp, {r0,r1}
-   11:          add     sp, sp, #2
-   12:          bal     - (9)
-   13:          mov     r0, r1
-   14:          sub     sp, fp, #2
-   15:          ldmfd   sp, {fp,sp,pc}
-Return:
-    r0
+    2:          sub     fp, ip, #1i
+    3:          cmp     r0, #0iw
+    4:          beq     + (7)
+    5:          sub     r3, r0, #1iw
+    6:          mul     r2, r0, r1
+    7:          stmfd   sp!, {r3,r2}
+    8:          ldmfd   sp, {r0,r1}
+    9:          add     sp, sp, #2i
+   10:          bal     - (7)
+   11:          mov     r0, r1
+   12:          sub     sp, fp, #3i
+   13:          ldmfd   sp, {fp,sp,pc}
 
  Initial goal:
-         !pc0 cpsr0 regs0 mems0.
-           (regs0 14 = 16w) /\ (regs0 13 = 100w) /\ (pc0 = 0) /\
-           terminated (instB,16) (pc0,cpsr0,regs0,mems0) ==>
-           (let (pc1,cpsr1,regs1,mems1) =
-                  terRun (instB,16) (pc0,cpsr0,regs0,mems0)
-            in
-              ((pc1 = 16) /\ T) /\
-              (read (regs1,mems1) (REG 0) =
-               f6 (read (regs0,mems0) (REG 0),read (regs0,mems0) (REG 1))))
-
-*)
+     !pc0 cpsr0 regs0 pc1 cpsr1 regs1 mems1.
+           ((regs0 ' 14 = 14w) /\ (regs0 ' 13 = 100w) /\ (pc0 = 0) /\
+            terminated (instB,14) (pc0,cpsr0,regs0,mems0)) /\
+           ((pc1,cpsr1,regs1,mems1) =
+            terRun (instB,14) (pc0,cpsr0,regs0,mems0)) ==>
+           (pc1 = 14) /\ (regs1 ' 0 = f6 (regs0 ' 0,regs0 ' 1))
 
 
-(*
     val env6 = toANF [] f6_def;
     val arm6 = compileEnv env6;
 	
@@ -237,15 +303,15 @@ THEN REWRITE_TAC []
     ] 		
 
 *)
+
 (*---------------------------------------------------------------------------*)
-(* Calling the Factorial Function                                            *)
+(* Example 5: Calling a recursive function				     *) 
+(* In this example, the Factorial Function is called                         *)
 (*---------------------------------------------------------------------------*)
 
 
-val (f7_def, f7_ind) = Defn.tprove
- (Hol_defn
-   "f7"
-   `f7 (x:num,a:num) = if x=0 then a else 
-	let k = x + 1 in f7(x-1,k*a)`,
-  WF_REL_TAC `measure FST`);
-
+val f7_def = Define
+   `f7 x =  
+	let t = f6 (x-1w, 1w) in
+	let k = t + t in
+	k`;
